refactor to prove tgts individually (for perf reasons)

src/certigrad/aevb/grads_correct.lean
@@ -8,25 +8,104 @@ applied to the naive variational encoder.
 -/
 import .util .naive ..prove_model_ok ..pre ..backprop_correct
 
-set_option max_memory 4096
+set_option max_memory 2048
 
 namespace certigrad
 namespace aevb
 
+set_option profiler true
 open graph list tactic certigrad.tactic
 
-theorem aevb_backprop_correct (a : arch) (ws : weights a) (x_data : T [a^.n_in, a^.n_x]) :
-let g := reparam (integrate_kl $ graph_naive a x_data) in
-let fdict := mk_input_dict ws g in
-∀ (tgt : reference) (idx : ℕ) (H_at_idx : at_idx g^.targets idx tgt),
+meta def prove_for_tgt : tactic unit :=
+do trace "prove_for_tgt start...",
+   whnf_target,
+
+/-
+   H_at_idx ← get_local `H_at_idx,
+   mk_app `and.right [H_at_idx] >>= note `H_tgt_eq,
+   H_tgt_eq_type ← get_local `H_tgt_eq >>= infer_type,
+   s ← join_user_simp_lemmas true [`cgsimp],
+   (H_tgt_eq_new_type, pr) ← simplify s H_tgt_eq_type {},
+   get_local `H_tgt_eq >>= λ H_tgt_eq, replace_hyp H_tgt_eq H_tgt_eq_new_type pr,
+   get_local `H_tgt_eq >>= subst,
+-/
+   applyc `certigrad.backprop_correct,
+   trace "targets subset inputs...",
+     solve1 cgsimp,
+   trace "at_idx...",
+     solve1 (applyc `and.intro >> dec_triv >> reflexivity),
+   trace "well_formed_at...",
+     solve1 (constructor >> all_goals cgsimp),
+   trace "grads_exist_at...",
+     solve1 (cgsimp),
+   trace "pdfs_exist_at...",
+     solve1 cgsimp,
+   trace "is_gintegrable...",
+     solve1 (cgsimp >> prove_is_mvn_integrable),
+   trace "can_diff_under_ints...",
+     solve1 (cgsimp >> prove_is_mvn_uintegrable),
+   trace "prove_for_tgt done"
+
+section params
+
+parameters (a : arch) (ws : weights a) (x_data : T [a^.n_in, a^.n_x])
+def g : graph := reparam (integrate_kl $ graph_naive a x_data)
+def fdict : env := mk_input_dict ws g
+
+attribute [cgsimp] g fdict
+
+lemma aevb_backprop_correct_W_encode :
+let idx := 0 in
+let tgt := (ID.str label.W_encode, [a^.ne, a^.n_in]) in
 ∇ (λ θ₀, E (graph.to_dist (λ m, ⟦sum_costs m g^.costs⟧) (env.insert tgt θ₀ fdict) g^.nodes) dvec.head) (env.get tgt fdict)
 =
 E (graph.to_dist (λ m, backprop g^.costs g^.nodes m g^.targets) fdict g^.nodes) (λ dict, dvec.get tgt.2 dict idx) :=
-by do whnf_target,
-      g ← to_expr ```(reparam (integrate_kl $ graph_naive a x_data)),
-      fdict ← to_expr ```(mk_input_dict ws (reparam (integrate_kl $ graph_naive a x_data))),
-      prove_model_ok g fdict
+by prove_for_tgt
 
+lemma aevb_backprop_correct_W_encode_μ :
+let idx := 1 in
+let tgt := (ID.str label.W_encode_μ, [a^.nz, a^.ne]) in
+∇ (λ θ₀, E (graph.to_dist (λ m, ⟦sum_costs m g^.costs⟧) (env.insert tgt θ₀ fdict) g^.nodes) dvec.head) (env.get tgt fdict)
+=
+E (graph.to_dist (λ m, backprop g^.costs g^.nodes m g^.targets) fdict g^.nodes) (λ dict, dvec.get tgt.2 dict idx) :=
+by prove_for_tgt
 
+lemma aevb_backprop_correct_W_encode_logσ₂ :
+let idx := 2 in
+let tgt := (ID.str label.W_encode_logσ₂, [a^.nz, a^.ne]) in
+∇ (λ θ₀, E (graph.to_dist (λ m, ⟦sum_costs m g^.costs⟧) (env.insert tgt θ₀ fdict) g^.nodes) dvec.head) (env.get tgt fdict)
+=
+E (graph.to_dist (λ m, backprop g^.costs g^.nodes m g^.targets) fdict g^.nodes) (λ dict, dvec.get tgt.2 dict idx) :=
+by prove_for_tgt
+
+lemma aevb_backprop_correct_W_decode :
+let idx := 3 in
+let tgt := (ID.str label.W_decode, [a^.nd, a^.nz]) in
+∇ (λ θ₀, E (graph.to_dist (λ m, ⟦sum_costs m g^.costs⟧) (env.insert tgt θ₀ fdict) g^.nodes) dvec.head) (env.get tgt fdict)
+=
+E (graph.to_dist (λ m, backprop g^.costs g^.nodes m g^.targets) fdict g^.nodes) (λ dict, dvec.get tgt.2 dict idx) :=
+by prove_for_tgt
+
+lemma aevb_backprop_correct_W_decode_p :
+let idx := 4 in
+let tgt := (ID.str label.W_decode_p, [a^.n_in, a^.nd]) in
+∇ (λ θ₀, E (graph.to_dist (λ m, ⟦sum_costs m g^.costs⟧) (env.insert tgt θ₀ fdict) g^.nodes) dvec.head) (env.get tgt fdict)
+=
+E (graph.to_dist (λ m, backprop g^.costs g^.nodes m g^.targets) fdict g^.nodes) (λ dict, dvec.get tgt.2 dict idx) :=
+by prove_for_tgt
+
+theorem aevb_backprop_correct :
+∀ (tgt : reference) (idx : ℕ) (H_at_idx : at_idx g^.targets idx tgt),
+∇ (λ θ₀, E (graph.to_dist (λ m, ⟦sum_costs m g^.costs⟧) (env.insert tgt θ₀ fdict) g^.nodes) dvec.head) (env.get tgt fdict)
+=
+E (graph.to_dist (λ m, backprop g^.costs g^.nodes m g^.targets) fdict g^.nodes) (λ dict, dvec.get tgt.2 dict idx)
+| tgt 0     H_at_idx := begin note H := and.right H_at_idx, subst H, apply aevb_backprop_correct_W_encode end
+| tgt 1     H_at_idx := begin note H := and.right H_at_idx, subst H, apply aevb_backprop_correct_W_encode_μ end
+| tgt 2     H_at_idx := begin note H := and.right H_at_idx, subst H, apply aevb_backprop_correct_W_encode_logσ₂ end
+| tgt 3     H_at_idx := begin note H := and.right H_at_idx, subst H, apply aevb_backprop_correct_W_decode end
+| tgt 4     H_at_idx := begin note H := and.right H_at_idx, subst H, apply aevb_backprop_correct_W_decode_p end
+| tgt (n+5) H_at_idx := false.rec _ $ list.at_idx_over H_at_idx dec_trivial
+
+end params
 end aevb
 end certigrad
